WIP mutual attestation

theories/examples/enclaves/mutual_attestation.v
@@ -4,58 +4,14 @@ Require Import Eqdep_dec List.
 From cap_machine Require Import rules seal_store.
 From cap_machine Require Import logrel fundamental.
 From cap_machine Require Import proofmode.
-From cap_machine Require Import macros_new.
+(* From cap_machine Require Import macros_new. *)
 Open Scope Z_scope.
-
-Section sealed_42.
-  Context {Σ:gFunctors} {ceriseg:ceriseG Σ} {sealsg: sealStoreG Σ}
-          {nainv: logrel_na_invs Σ} `{MP: MachineParameters}.
-
-  Program Definition f42 : Addr := (finz.FinZ 42 eq_refl eq_refl).
-  Definition sealed_42 : LWord → iProp Σ :=
-    λ w, (∃ b e v, ⌜w = LCap O b e f42 v⌝)%I.
-  Definition sealed_42_ne : (leibnizO LWord) -n> (iPropO Σ) :=
-      λne (w : leibnizO LWord), sealed_42 w%I.
-
-  Instance sealed_42_persistent (w : LWord) : Persistent (sealed_42 w).
-  Proof. apply _. Qed.
-
-  Definition seal_pred_42 (τ : OType) := seal_pred τ sealed_42.
-  Definition valid_sealed_42_cap (w : LWord) (τ : OType) := valid_sealed w τ sealed_42.
-  Lemma sealed_42_interp (lw : LWord) : sealed_42 lw -∗ fixpoint interp1 lw.
-  Proof.
-    iIntros "Hsealed". iDestruct "Hsealed" as (b e v) "->".
-    by rewrite fixpoint_interp1_eq /=.
-  Qed.
-End sealed_42.
-
-Section sealed_43.
-  Context {Σ:gFunctors} {ceriseg:ceriseG Σ} {sealsg: sealStoreG Σ}
-          {nainv: logrel_na_invs Σ} `{MP: MachineParameters}.
-
-  Program Definition f43 : Addr := (finz.FinZ 43 eq_refl eq_refl).
-  Definition sealed_43 : LWord → iProp Σ :=
-    λ w, (∃ b e v, ⌜w = LCap O b e f43 v⌝)%I.
-  Definition sealed_43_ne : (leibnizO LWord) -n> (iPropO Σ) :=
-      λne (w : leibnizO LWord), sealed_43 w%I.
-
-  Instance sealed_43_persistent (w : LWord) : Persistent (sealed_43 w).
-  Proof. apply _. Qed.
-
-  Definition seal_pred_43 (τ : OType) := seal_pred τ sealed_43.
-  Definition valid_sealed_43_cap (w : LWord) (τ : OType) := valid_sealed w τ sealed_43.
-  Lemma sealed_43_interp (lw : LWord) : sealed_43 lw -∗ fixpoint interp1 lw.
-  Proof.
-    iIntros "Hsealed". iDestruct "Hsealed" as (b e v) "->".
-    by rewrite fixpoint_interp1_eq /=.
-  Qed.
-End sealed_43.
-
 
 Section mutual_attest_example.
   Context {Σ:gFunctors} {ceriseg:ceriseG Σ} {sealsg : sealStoreG Σ}
     {nainv: logrel_na_invs Σ} `{MP: MachineParameters}.
-  Context (assert_entry_point : LWord).
+  Context (malloc_entry_point : LWord).
+  Context (ma_addr_A ma_addr_B : Addr).
 
   (* -------------------------------------- *)
   (* ------ MUTUAL ATTEST *ENCLAVES* ------ *)
@@ -65,20 +21,72 @@ Section mutual_attest_example.
      - r_t0 contains return pointer to adv
      - r_t1 contains entry point to ENCLAVE B, not attested yet
    *)
-  Definition mutual_attest_enclave_A_code_pre : list LWord :=
+  (* Dynamic check:
+     data[0] = #A
+     data[1] = #A
+     data[2] = malloc_entry_point
+   *)
+  Definition mutual_attest_enclave_A_code : list LWord :=
     encodeInstrsLW [
+
+      (* fetch ?malloc *)
+      (* hash ?malloc *)
+      (* if #?malloc =! #malloc_entry_point --> fail *)
+
+      (* malloc a buffer b of size 3:
+         will be used to communicate
+      *)
+
+      (* let idA := hash PC[1::-] *)
+      (* let idT := data[0-1] *)
+
+      (* if idA != idT, then fail *)
+
+      (* hash idT *)
+
+      (* let mbA := base(b) % 3 *)
+      (* if mbA == 0,
+         then we can use
+         + mbA[0] for #idT
+         + mbA[1] for 42    // attestation of A for B
+         + mbA[2] for 1     // attestation of A for main
+       *)
+      (* if mbA == 1,
+         then we can use
+         + mbA[0] for 1     // attestation of A for main
+         + mbA[1] for #idT
+         + mbA[2] for 42    // attestation of A for B
+       *)
+      (* if mbA == 2,
+         then we can use
+         + mbA[0] for 42    // attestation of A for B
+         + mbA[1] for 1     // attestation of A for main
+         + mbA[2] for #idT
+       *)
+
       (* fetch sign key *)
-      (* signs {42}_signed_A *)
+      (* signs { mbA[#idT] }_signed_A *)
+      (* signs { mbA[w42] }_signed_A *)
+
       (* call ENCLAVE B with
-        r_t1 := {42}_signed_A;
-        r_t2 := pub_sign_key_A;
+        r_t30 := return pointer;
+        r_t1  := { mbA[#idT] }_signed_A;
+        r_t2  := { mbA[w42] }_signed_A;
+        r_t3  := pub_sign_key_A;
       *)
 
       (* ---- we only arrive here if B has successfully attested A ---- *)
       (* receives:
-         r_t1 := {43}_signed_B;
-         r_t2 := pub_sign_key_B;
+        r_t1  := { mbB[#idT] }_signed_B;
+        r_t2  := { mbB[w43] }_signed_B;
+        r_t3  := pub_sign_key_B;
       *)
+
+      (* ATTEST B *)
+      (* TODO @June: how do I attest
+         the value returned by B
+      *)
+      (* if mbA[#idT] != mbB[#idT], then fail *)
 
       (* CHECK ATTESTS B *)
       (* get idT(B) in r_t2 *)
@@ -91,14 +99,13 @@ Section mutual_attest_example.
 
       Jmp r_t0
       (* REST OF CODE OF A *)
-    ]
-    ++ [assert_entry_point].
+    ].
 
   (* Expects:
      - r_t0 contains return pointer to caller
      - r_t1 contains entry point to ENCLAVE B, not attested yet
    *)
-  Definition mutual_attest_enclave_B_code_pre : list LWord :=
+  Definition mutual_attest_enclave_B_code : list LWord :=
     encodeInstrsLW [
       (* CODE INITIALISATION ENCLAVE B *)
 
@@ -123,64 +130,163 @@ Section mutual_attest_example.
         r_t2 := pub_sign_key_B;
       *)
       Jmp r_t0
-    ]
-    ++ [assert_entry_point].
-
-  Definition mutual_attest_eid_table : list LWord :=
-    [
-      LWInt (hash (mutual_attest_enclave_A_code_pre));
-      LWInt (hash (mutual_attest_enclave_B_code_pre))
     ].
 
-  Definition mutual_attest_enclave_A_code : list LWord :=
-    mutual_attest_enclave_A_code_pre ++ mutual_attest_eid_table .
+  Definition hash_mutual_attest_A : Z :=
+    (hash_concat (hash ma_addr_A) (hash mutual_attest_enclave_A_code)).
+  Definition hash_mutual_attest_B : Z :=
+    (hash_concat (hash ma_addr_B) (hash mutual_attest_enclave_B_code)).
 
-  Definition mutual_attest_enclave_B_code : list LWord :=
-    mutual_attest_enclave_B_code_pre ++ mutual_attest_eid_table .
+  Definition mutual_attest_eid_table : list LWord :=
+    [ LWInt hash_mutual_attest_A; LWInt hash_mutual_attest_B ].
 
   Definition mutual_attest_enclave_A (enclave_data_cap : LWord) : list LWord :=
-    enclave_data_cap::(mutual_attest_enclave_A_code ).
+    enclave_data_cap::mutual_attest_enclave_A_code.
 
   Definition mutual_attest_enclave_B (enclave_data_cap : LWord) : list LWord :=
-    enclave_data_cap::(mutual_attest_enclave_B_code ).
+    enclave_data_cap::mutual_attest_enclave_B_code.
 
-  Definition hash_mutual_attest_enclave_A (tc_addr : Addr) : Z :=
-    hash_concat (hash tc_addr) (hash mutual_attest_enclave_A_code).
+  Definition mutual_attestN : namespace := nroot .@ "mutual_attest".
 
-  Definition hash_mutual_attest_enclave_B (tc_addr : Addr) : Z :=
-    hash_concat (hash tc_addr) (hash mutual_attest_enclave_B_code).
+  Axiom hash_pos : forall {A : Type} (a : A), hash a >= 0.
+
+  (* Sealed predicate for enclave A *)
+  Definition prot_sealed_A (a : Addr) (lw : LWord) : iProp Σ:=
+    ⌜ if (decide (a `mod` 3 = 0 ))
+      then
+        ( (∃ (w' : LWord), lw = LInt (hash [LInt hash_mutual_attest_A; w'])) )
+      else
+        if (decide (a `mod` 3 = 1 ))
+        then lw = LInt 42
+        else lw = LInt 1 ⌝%I.
+
+  Definition sealed_enclaveA : LWord → iProp Σ :=
+    λ w, (∃ a v,
+             ⌜ w = LCap RO a (a^+1)%a a v ⌝
+             ∗ ⌜(a+1)%a = Some (a^+1)%a ⌝
+             ∗ (inv (logN.@(a, v)) (∃ lw, (a,v) ↦ₐ lw ∗ prot_sealed_A a lw)))%I.
+  Definition sealed_enclaveA_ne : (leibnizO LWord) -n> (iPropO Σ) :=
+      λne (w : leibnizO LWord), sealed_enclaveA w%I.
+
+  Instance sealed_enclaveA_persistent (w : LWord) : Persistent (sealed_enclaveA w).
+  Proof. apply _. Qed.
+
+  Definition seal_pred_enclaveA (τ : OType) := seal_pred τ sealed_enclaveA.
+  Definition valid_sealed_enclaveA_cap (w : LWord) (τ : OType) := valid_sealed w τ sealed_enclaveA.
+  Lemma sealed_enclaveA_interp (lw : LWord) : sealed_enclaveA lw -∗ fixpoint interp1 lw.
+  Proof.
+    iIntros "Hsealed".
+    iDestruct "Hsealed" as (a v -> HB) "Hinv".
+    rewrite fixpoint_interp1_eq /=.
+    rewrite finz_seq_between_singleton; auto.
+    iApply big_sepL_singleton.
+    iExists (λne (lw : leibnizO LWord), prot_sealed_A a lw).
+    iFrame "Hinv".
+    iSplit.
+    - iPureIntro. intros lw. apply _.
+    - iNext ; iModIntro.
+      iIntros (lw Hlw); cbn.
+      destruct (decide (a `mod` 3 = 0)); first (destruct Hlw as [n Hlw] ; simplify_eq; by rewrite fixpoint_interp1_eq).
+      destruct (decide (a `mod` 3 = 1)); simplify_eq; by rewrite fixpoint_interp1_eq.
+  Qed.
+
+
+  (* Sealed predicate for enclave B *)
+  Definition prot_sealed_B (a : Addr) (lw : LWord) : iProp Σ:=
+    ⌜ if (decide ( a `mod` 2 = 0 ) )
+      then lw = LInt (hash [LInt hash_mutual_attest_A; LInt hash_mutual_attest_B])
+      else lw = LInt 43 ⌝%I.
+
+  Definition sealed_enclaveB : LWord → iProp Σ :=
+    λ w, (∃ a v,
+             ⌜ w = LCap RO a (a^+1)%a a v ⌝
+             ∗ ⌜(a+1)%a = Some (a^+1)%a ⌝
+             ∗ (inv (logN.@(a, v)) (∃ lw, (a,v) ↦ₐ lw ∗ prot_sealed_B a lw)))%I.
+  Definition sealed_enclaveB_ne : (leibnizO LWord) -n> (iPropO Σ) :=
+      λne (w : leibnizO LWord), sealed_enclaveB w%I.
+
+  Instance sealed_enclaveB_persistent (w : LWord) : Persistent (sealed_enclaveB w).
+  Proof. apply _. Qed.
+
+  Definition seal_pred_enclaveB (τ : OType) := seal_pred τ sealed_enclaveB.
+  Definition valid_sealed_enclaveB_cap (w : LWord) (τ : OType) := valid_sealed w τ sealed_enclaveB.
+  Lemma sealed_enclaveB_interp (lw : LWord) : sealed_enclaveB lw -∗ fixpoint interp1 lw.
+  Proof.
+    iIntros "Hsealed".
+    iDestruct "Hsealed" as (a v -> HB) "Hinv".
+    rewrite fixpoint_interp1_eq /=.
+    rewrite finz_seq_between_singleton; auto.
+    iApply big_sepL_singleton.
+    iExists (λne (lw : leibnizO LWord), prot_sealed_B a lw).
+    iFrame "Hinv".
+    iSplit.
+    - iPureIntro. intros lw. apply _.
+    - iNext ; iModIntro.
+      iIntros (lw Hlw); cbn.
+      destruct (decide (a `mod` 2 = 0)); simplify_eq; by rewrite fixpoint_interp1_eq.
+  Qed.
+
 
   (* Trusted Compute Custom Predicates *)
-  Definition mutual_attest_enclave_A_pred (ma_addr_A : Addr) : CustomEnclave :=
+  Definition mutual_attest_enclave_A_pred : CustomEnclave :=
     @MkCustomEnclave Σ
       mutual_attest_enclave_A_code
       ma_addr_A
       (λ w, False%I)
-      sealed_42.
-  Definition mutual_attest_enclave_B_pred (ma_addr_B : Addr) : CustomEnclave :=
+      sealed_enclaveA.
+  Definition mutual_attest_enclave_B_pred : CustomEnclave :=
     @MkCustomEnclave Σ
       mutual_attest_enclave_B_code
       ma_addr_B
       (λ w, False%I)
-      sealed_43.
+      sealed_enclaveB.
 
-  Definition ma_enclaves_map (ma_addr_A ma_addr_B : Addr) : custom_enclaves_map :=
-   {[ hash_mutual_attest_enclave_A ma_addr_A := mutual_attest_enclave_A_pred ma_addr_A;
-      hash_mutual_attest_enclave_B ma_addr_B := mutual_attest_enclave_B_pred ma_addr_B
+  Definition ma_enclaves_map : custom_enclaves_map :=
+   {[ hash_mutual_attest_A := mutual_attest_enclave_A_pred;
+      hash_mutual_attest_B := mutual_attest_enclave_B_pred
    ]}.
 
-  Lemma wf_ma_enclaves_map (ma_addr_A ma_addr_B : Addr) :
-    custom_enclaves_map_wf (ma_enclaves_map ma_addr_A ma_addr_B).
+  Lemma wf_ma_enclaves_map :
+    custom_enclaves_map_wf ma_enclaves_map.
   Proof.
     rewrite /custom_enclaves_map_wf /ma_enclaves_map.
     apply (map_Forall_insert_2 (λ (I : Z) (ce : CustomEnclave), _)).
-    - by rewrite /hash_mutual_attest_enclave_A /=.
-    - by rewrite map_Forall_singleton /hash_mutual_attest_enclave_B /=.
+    - by rewrite /hash_mutual_attest_A /=.
+    - by rewrite map_Forall_singleton /hash_mutual_attest_B /=.
   Qed.
 
-  Lemma tc_contract (ma_addr_A ma_addr_B : Addr) :
-    custom_enclave_contract (ma_enclaves_map ma_addr_A ma_addr_B).
+
+
+  Lemma mutual_attest_contract :
+    custom_enclave_contract ma_enclaves_map.
   Proof.
+    rewrite /custom_enclave_contract.
+    iIntros (I b e a v b' e' a' v' enclave_data ot ce
+      Hwf_cemap Hcode_ce Hot Hb' Hwfbe HIhash Hb He)
+      "(#Henclaves_inv & #Hma_inv & #HPenc & #HPsign)".
+    clear HIhash.
+
+    rewrite /ma_enclaves_map in Hcode_ce.
+    simplify_map_eq.
+
+    assert (I = hash_mutual_attest_A \/ I = hash_mutual_attest_B) as HI.
+    { rewrite lookup_insert_Some in Hcode_ce.
+      destruct Hcode_ce as [ [? _] | [_ Hcode_ce] ]; first auto.
+      rewrite lookup_insert_Some in Hcode_ce.
+      destruct Hcode_ce as [ [? _] | [_ Hcode_ce] ]; first auto.
+      done.
+    }
+    destruct HI ; simplify_map_eq.
+    - rewrite fixpoint_interp1_eq /=.
+      iIntros (lregs); iNext ; iModIntro.
+      iIntros "([%Hfullmap #Hinterp_map] & Hrmap & Hna)".
+      rewrite /interp_conf.
+      iMod (na_inv_acc with "Hma_inv Hna") as "(>[Hma_code Htc_data]  & Hna & Hclose)"; [solve_ndisj ..|].
+      rewrite /registers_mapsto.
+      iExtract "Hrmap" PC as "HPC".
+      remember ma_addr_A as pc_b in |- * at 7.
+      remember (ma_addr_A ^+ (1%nat + 1))%a as pc_e in |- * at 4.
+      (* assert (SubBounds pc_b pc_e ma_addr_A (ma_addr_A ^+ (4%nat + 1))%a) by (subst; solve_addr). *)
   Admitted.
 
 End mutual_attest_example.
